Implementa is_empty, top e push

Stack.dfy
@@ -1,22 +1,75 @@
-/**********************
-    INTEGRANTES
-    
-    Douglas Dallavale
-    Douglas Paz
-    João Viera
-**********************/
+class Stack {
+  var arr : array<int>;
+  var index : nat;
+  ghost var elements: seq<int>;
+  predicate Valid() reads this
+  {
+    0 <= index < arr.Length
+  }
 
-class Stack
-{
-  var arr: array<int>
-  
-  constructor(size: nat) ensures arr.Length == size
+  predicate Empty() reads this
+  {
+    index == 0
+  }
+  predicate Full() reads this
+  {
+    index == arr.Length
+  }
+
+  constructor(size: nat) 
+    requires size > 0 
+    ensures Valid()
+    ensures Empty()
+    ensures fresh(arr)
+    ensures arr.Length == size
   {
     arr := new int[size];
+    elements := [];
+    index := 0;
+  }
+
+  method IsEmpty() returns (result : bool)
+    requires Empty()
+  {
+      return true;
+  }
+
+  method Top()
+    returns (element: int) 
+    requires Valid()
+    requires !Empty()
+    ensures element == arr[index]
+    ensures index == old(index)
+  {
+    element := arr[index];
+  }
+
+  method Push(element : int) 
+    modifies arr, `index
+    requires Valid()
+    requires !Full()
+    ensures index == old(index) + 1
+  {
+      arr[index] := element;
+      index := index+1;
+  }
+
+  method Pop() returns (elem : int)
+  {
   }
 }
 
+
 method Main()
 {
-  
+  var stack := new Stack(4);
+  stack.Push(1);
+  stack.Push(2);
+  stack.Push(3);
+  stack.Push(3);
+
+  //result := stack.Push(5);
+  //result := stack.Push(5);
+
+  //result := stack.Push(5);
 }
